seiostar/LogRelTargetSource.CompatibilityLemmas.fst
@@ -13,7 +13,7 @@ let bind_squash (a #b:Type) (f:a -> GTot (squash b)) : Pure (squash b) (requires
 
 let get_squash = FStar.Squash.get_proof
 
-let compat_oval_unit g : Lemma (fs_oval_return g qUnit () ⊐ EUnit) =
+let compat_oval_unit g : Lemma (fs_oval_return g #qUnit () ⊐ EUnit) =
   introduce forall b (s:gsub g b) fsG h. fsG `(∽) h` s ==> qUnit ⊇ (h, (), gsubst s EUnit) with begin
     introduce _ ==> _ with _. begin
       assert (qUnit ∋ (h, (), EUnit));
@@ -21,7 +21,7 @@ let compat_oval_unit g : Lemma (fs_oval_return g qUnit () ⊐ EUnit) =
     end
   end
 
-let compat_oval_true g : Lemma (fs_oval_return g qBool true ⊐ ETrue) =
+let compat_oval_true g : Lemma (fs_oval_return g #qBool true ⊐ ETrue) =
   introduce forall b (s:gsub g b) fsG h. fsG `(∽) h` s ==> qBool ⊇ (h, true, gsubst s ETrue) with begin
     introduce _ ==> _ with _. begin
       assert (qBool ∋ (h, true, ETrue));
@@ -29,7 +29,7 @@ let compat_oval_true g : Lemma (fs_oval_return g qBool true ⊐ ETrue) =
     end
   end
 
-let compat_oval_false g : Lemma (fs_oval_return g qBool false ⊐ EFalse) =
+let compat_oval_false g : Lemma (fs_oval_return g #qBool false ⊐ EFalse) =
   introduce forall b (s:gsub g b) fsG h. fsG `(∽) h` s ==> qBool ⊇ (h, false, gsubst s EFalse) with begin
     introduce _ ==> _ with _. begin
       assert (qBool ∋ (h, false, EFalse));
@@ -37,7 +37,7 @@ let compat_oval_false g : Lemma (fs_oval_return g qBool false ⊐ EFalse) =
     end
   end
 
-let compat_oval_file_descr g fd : Lemma (fs_oval_return g qFileDescr fd ⊐ EFileDescr fd) =
+let compat_oval_file_descr g fd : Lemma (fs_oval_return g #qFileDescr fd ⊐ EFileDescr fd) =
   introduce forall b (s:gsub g b) fsG h. fsG `(∽) h` s ==> qFileDescr ⊇ (h, fd, gsubst s (EFileDescr fd)) with begin
     introduce _ ==> _ with _. begin
       assert (qFileDescr ∋ (h, fd, (EFileDescr fd)));
@@ -45,7 +45,7 @@ let compat_oval_file_descr g fd : Lemma (fs_oval_return g qFileDescr fd ⊐ EFil
     end
   end
 
-let compat_oval_string g (str:string) : Lemma (fs_oval_return g qString str ⊐ EString str) =
+let compat_oval_string g (str:string) : Lemma (fs_oval_return g #qString str ⊐ EString str) =
   introduce forall b (s:gsub g b) fsG h. fsG `(∽) h` s ==> qString ⊇ (h, str, gsubst s (EString str)) with begin
     introduce _ ==> _ with _. begin
       assert (qString ∋ (h, str, EString str));
@@ -618,7 +618,7 @@ let compat_oval_lambda_oprod #g (#t1:qType) (#t2:qType) (fs_body:fs_oprod (exten
 let compat_oprod_return #g (#t:qType) (fs_x:fs_oval g t) (x:exp)
   : Lemma
     (requires fs_x ⊐ x)
-    (ensures fs_oprod_return fs_x ⊒ x) =
+    (ensures fs_oprod_return_oval fs_x ⊒ x) =
   introduce forall b (s:gsub g b) fsG h. fsG `(∽) h` s ==> t ⫄ (h, return (fs_x fsG), gsubst s x) with begin
     introduce _ ==> _ with _. begin
       let fs_x = fs_x fsG in
@@ -1085,19 +1085,19 @@ let compat_oprod_close_oval #g (fs_fd:fs_oval g qFileDescr) (fd:exp)
 
 let compat_oprod_unit g : Lemma (fs_oprod_return_val g qUnit () ⊒ EUnit) =
   compat_oval_unit g;
-  compat_oprod_return (fs_oval_return g qUnit ()) EUnit
+  compat_oprod_return (fs_oval_return g #qUnit ()) EUnit
 
 let compat_oprod_true g : Lemma (fs_oprod_return_val g qBool true ⊒ ETrue) =
   compat_oval_true g;
-  compat_oprod_return (fs_oval_return g qBool true) ETrue
+  compat_oprod_return (fs_oval_return g #qBool true) ETrue
 
 let compat_oprod_false g : Lemma (fs_oprod_return_val g qBool false ⊒ EFalse) =
   compat_oval_false g;
-  compat_oprod_return (fs_oval_return g qBool false) EFalse
+  compat_oprod_return (fs_oval_return g #qBool false) EFalse
 
 let compat_oprod_string g s : Lemma (fs_oprod_return_val g qString s ⊒ EString s) =
   compat_oval_string g s;
-  compat_oprod_return (fs_oval_return g qString s) (EString s)
+  compat_oprod_return (fs_oval_return g #qString s) (EString s)
 
 open FStar.Tactics.V1
 
@@ -1146,7 +1146,7 @@ let compat_oprod_if #g
 
 let compat_oprod_file_descr g fd : Lemma (fs_oprod_return_val g qFileDescr fd ⊒ EFileDescr fd) =
   compat_oval_file_descr g fd;
-  compat_oprod_return (fs_oval_return g qFileDescr fd) (EFileDescr fd)
+  compat_oprod_return (fs_oval_return g #qFileDescr fd) (EFileDescr fd)
 
 let compat_oprod_var g (x:var{Some? (g x)}) : Lemma (fs_oprod_var g x ⊒ EVar x) =
   compat_oval_var g x;
@@ -1715,7 +1715,7 @@ let compat_oprod_write #g (fs_fd:fs_oprod g qFileDescr) (fs_msg:fs_oprod g qStri
       let fs_pair' = fs_prod_bind fs_fd' (fun x' -> fs_prod_bind #qString #(qFileDescr ^* qString) fs_msg' (fun y' -> return (x', y'))) in
       let fs_e = fs_prod_bind fs_pair' (fun args' -> io_call OWrite args') in
       assert (fs_e == (fs_oprod_call OWrite (fs_oprod_pair fs_fd fs_msg)) fsG) by (
-        norm [delta_only [`%fs_oprod_call;`%fs_oprod_pair;`%fs_oprod_bind';`%fs_oprod_bind;`%fs_oprod_return_prod;`%fs_oprod_return_val;`%fs_val_pair;`%fs_prod_bind]];
+        norm [delta_only [`%fs_oprod_call;`%fs_oprod_pair;`%fs_oprod_bind';`%fs_oprod_bind;`%fs_oprod_return;`%fs_oprod_return_val;`%fs_val_pair;`%fs_prod_bind]];
         l_to_r [`lem_hd_stack;`tail_stack_inverse];
         trefl ());
       let e = EWrite (gsubst s fd) (gsubst s msg) in
