seiostar/QTypes.fst
@@ -81,3 +81,20 @@ let (^+) (t1 t2:qType) : qType =
   (| _, QSum (get_rel t1) (get_rel t2) |)
 
 let qResexn (t1:qType) : qType = t1 ^+ qUnit
+
+
+unfold
+let q_io_args (o:io_ops) : qType =
+  match o with
+  | OOpen  -> qString
+  | ORead  -> qFileDescr
+  | OWrite -> qFileDescr ^* qString
+  | OClose -> qFileDescr
+
+unfold
+let q_io_res (o:io_ops) : qType =
+  match o with
+  | OOpen  -> qResexn qFileDescr
+  | ORead  -> qResexn qString
+  | OWrite -> qResexn qUnit
+  | OClose -> qResexn qUnit
